

let $X \in \mathcal{X}(M)$. let us start at point $p \in M$ now we want to find a curve $\gamma: (-\varepsilon, \varepsilon) \rightarrow M$ with $\gamma(0) = p$ and $\gamma'(t) = X_{\gamma(t)} \Leftrightarrow d\gamma \left(\frac{d}{dt} \Big|_{t=t_0} \right) = X_{\gamma(t_0)}$

$$\Leftrightarrow \forall f \in C^\infty(M): \frac{d}{dt} \Big|_{t=t_0} (f \circ \gamma)(t) = X_{\gamma(t_0)} f$$

So such curve is called an integral curve of X through p .

let (U, φ) be coordinates around p . In these coordinates $X = X^i \frac{\partial}{\partial x^i}$ and $\gamma(t) = (\gamma^1(t), \dots, \gamma^n(t))$

and $\gamma^i: (-\varepsilon, \varepsilon) \rightarrow \mathbb{R}$. $\gamma'(t) = \gamma^{i'}(t) \frac{\partial}{\partial x^i}$ hence we get a system of ODEs $\gamma^{i'}(t) = X^i(\gamma(t))$

\Rightarrow solution exists for some small neighbourhood of p .

Hence we have a map $\varphi_x: (-\varepsilon, \varepsilon) \times V \rightarrow M$ s.t. for any fixed q the map $\varphi_x^q: (-\varepsilon, \varepsilon) \rightarrow M$ is the integral curve of X through q .
 \uparrow
 where the solution exists around p

we say X is a complete vector field if the flow at all points exists for all time.

let $f: X \rightarrow \mathbb{R}$ be a function then $\text{supp } f = \overline{\{p \in X \mid f(p) \neq 0\}}$

If $X \in \mathcal{X}(M)$ and $\text{supp } X$ is compact then X is complete.

\Rightarrow If M is compact then every vector field has complete flow.

Examples: (i) let $X = x^2 \frac{d}{dx}$ on \mathbb{R} then an integral curve must satisfy $\gamma' = \gamma^2$

$\Rightarrow \gamma(t) = \frac{1}{c-t}$ where $c = \frac{1}{\gamma(0)}$. Note: at $x=0 \Rightarrow X|_0 = 0$ and so at 0 it has complete flow.

ii) let $X = x \frac{d}{dx}$ then $\gamma_x^p(t) = pe^t \Rightarrow \varphi_x(t, p) = pe^t$.

let $X \in \mathcal{X}(M)$ with flow defined on $\varphi_x: J \rightarrow M$ where $J = \{(t, p) \mid \text{the integral curve through } p \text{ exists at } t\}$
 Then note that $(t, \varphi_x(s, p)) \in J \Leftrightarrow (t+s, p) \in J$ moreover $\varphi_x(t+s, p) = \varphi_x(t, \varphi_x(s, p))$
 flow property.

Proof: Let $f \in C^\infty(M)$ then $\frac{d}{dt} f(\varphi_x(t+s, p)) = \frac{d}{d\tau} \Big|_{\tau=t+s} f(\varphi_x(\tau, p)) = X_{\varphi_x(t+s, p)}(f)$

Hence by uniqueness $\varphi_x(t+s, p) = \varphi_x(t, \varphi_x(s, p))$.

Note: $\varphi_x(0, p) = p \Rightarrow \varphi_x^0 = \text{id}_M$ hence φ_x^t is a diffeomorphism of its domain. Since φ_x^{-t} is its inverse.

If X is complete we get smooth action of \mathbb{R} on M . $t \mapsto \varphi_x^t$

Let X and $Y \in \mathfrak{X}(M)$. Is $X \circ Y$ a vector field?

$$\begin{aligned} \text{Let } f \in C^\infty(M) \text{ then } X(Yf) &= X^i \partial_i (Y^j \partial_j f) \\ &= X^i \partial_i Y^j \partial_j f + X^i Y^j \partial_i \partial_j f \end{aligned}$$

$$\begin{aligned} Y(Xf) &= Y^j \partial_j (X^i \partial_i f) \\ &= Y^j \partial_j X^i \partial_i f + X^i Y^j \partial_j \partial_i f \end{aligned}$$

Hence $[X, Y]f = X(Yf) - Y(Xf) \stackrel{!}{=} \text{a vector field. This is the Lie bracket of } X \text{ and } Y.$

Suppose $F: M \rightarrow N$ is a diffeomorphism $\Rightarrow F^*f: M \rightarrow \mathbb{R}$
 $p \mapsto f(F(p))$

$$\begin{array}{ccc} C^\infty(M) & \xrightarrow{F^*} & C^\infty(N) \\ F^* \uparrow & \circlearrowleft & \uparrow F^* \\ C^\infty(N) & \xrightarrow{F} & C^\infty(M) \end{array}$$

$$(F^*Y)(F^*g) = F^*(Y(g)) \Leftrightarrow (F^*Y)_p = dF_p^{-1}(Y_{F(p)})$$

$$\begin{aligned} F: p &\mapsto F(p) \\ T_p M &\mapsto T_{F(p)} N \end{aligned}$$

$$\begin{aligned} F^!: P(p) &\mapsto P \\ T_{F(p)} N &\mapsto T_p M \end{aligned}$$

$$F^*[X, Y] = [F^*X, F^*Y]$$

Let $X \in \mathfrak{X}(M)$ be complete $(\varphi_x^t)^*: \mathfrak{X}(M) \rightarrow \mathfrak{X}(M)$
 $Y \mapsto (\varphi_x^t)^* Y$

$$\mathcal{L}_X f = \frac{d}{dt} \Big|_{t=0} (\varphi_x^t)^* f = \frac{d}{dt} \Big|_{t=0} f \circ \varphi_x^t \leftarrow \text{Lie derivative of } f \text{ wrt } X.$$

$$\mathcal{L}_X Y = \frac{d}{dt} \Big|_{t=0} (\varphi_x^t)^* Y$$

Theorem: let $X, Y \in \mathcal{X}(M)$ then $\mathcal{L}_X Y = [X, Y]$

Proof: $(\varphi_x^t)^*(Y(f)) = (\varphi_x^t)^* Y((\varphi_x^t)^* f)$ take derivative at $t=0$

$$\begin{aligned} X(Y(f)) &= \left(\frac{d}{dt} \bigg|_{t=0} (\varphi_x^t)^* Y \right)(f) + Y \left(\frac{d}{dt} \bigg|_{t=0} (\varphi_x^t)^* f \right) \\ &= (\mathcal{L}_X Y)(f) + Y(Xf) \end{aligned}$$

$$\Rightarrow \mathcal{L}_X Y = [X, Y]$$

$$\text{Note } \mathcal{L}_X Y = -\mathcal{L}_Y X$$